Splinter/Paged/Bundle.i.dfy
@@ -1,10 +1,11 @@
 include "AbstractJournal.i.dfy"
+include "AbstractMap.i.dfy"
 include "PagedJournal.i.dfy"
 
 // Hey look, this abstract journal satisfies the refinement.
-module AbstractJournalRefinement refines CoordinationSystemRefinement(AbstractJournal) {
+module AbstractJournalRefinement refines CoordinationSystemRefinement(AbstractJournal, AbstractMap) {
 }
 
 // Ooh, and so does this Paged journal
-module PagedJournalRefinement refines CoordinationSystemRefinement(PagedJournal) {
+module PagedJournalRefinement refines CoordinationSystemRefinement(PagedJournal, AbstractMap) {
 }
