Splinter/Paged/LinkedJournal.i.dfy
@@ -1,0 +1,37 @@
+
+
+module LinkedJournal {
+  type Pointer = nat
+
+  datatype JournalRecord = JournalRecord(
+    messageSeq: MsgHistory,
+    priorRec: Option<Pointer>
+  )
+  {
+    function I(cacheView: CacheView) : PagedJournalIfc.JournalRecord
+    {
+      PagedJournalIfc.JournalRecord(messageSeq,
+        if priorRec.None?
+        then None
+        else if priorRec.value !in cacheView
+        then None
+        else Some(cacheView[priorRec.value].I(cacheView))
+      )
+    }
+  }
+
+  type CacheView = map<Pointer, JournalRecord>
+
+  datatype TruncatedJournal = TruncatedJournal(
+    boundaryLSN : LSN,  // exclusive: lsns <= boundaryLSN are discarded
+    freshestRec: Option<Pointer>,
+    cacheView: CacheView)
+  {
+    function I() : PagedJournalIfc.TruncatedJournal
+    {
+  
+    }
+  }
+
+
+}
